x86/FlatAsmgenproof.v
@@ -5,7 +5,7 @@
 
 (** Correctness proof for the FlatAsm generation **)
 
-Require Import Coqlib Integers Values.
+Require Import Coqlib Integers Values Maps AST.
 Require Import Memtype Memory.
 Require Import Asm RawAsmgen.
 Require Import FlatAsm FlatAsmgen.
@@ -15,7 +15,6 @@ Require Import StackADT.
 Require Import Linking Errors.
 Require Import Globalenvs FlatAsmGlobenv.
 Require Import RawAsmgen.
-Require Import Sectinj.
 
 Section WITHMEMORYMODEL.
   
@@ -38,11 +37,63 @@ Let tge := globalenv tprog.
 Definition regset_inject (j:meminj) (rs rs' : regset) : Prop :=
   forall r, Val.inject j (rs r) (rs' r).
 
+(** Agreement between a memory injection from Asm to the flat memory and 
+    the mappings for sections, global id and labels *)    
+Record match_sminj (gm: GID_MAP_TYPE) (lm: LABEL_MAP_TYPE) (sm: section_map) (mj: meminj) : Type :=
+  mk_match_sminj {
+      (* agree_sminj : forall b id sid ofs ofs',  *)
+      (*   Genv.find_symbol ge id = Some b -> *)
+      (*   gm id = Some (sid,ofs) -> PTree.get sid sm = Some ofs' ->  *)
+      (*   mj b = Some (mem_block, Ptrofs.unsigned (Ptrofs.add ofs ofs')); *)
+ 
+      agree_sminj_instr :  forall b b' f ofs ofs' i,
+          Genv.find_funct_ptr ge b = Some (Internal f) -> 
+          Asm.find_instr (Ptrofs.unsigned ofs) (Asm.fn_code f) = Some i ->
+          mj b = Some (b', ofs') -> 
+          exists id i' ofs1, 
+            Genv.find_instr tge (Ptrofs.add ofs (Ptrofs.repr ofs')) = Some i' /\
+            Genv.find_symbol ge id = Some b /\
+            transl_instr gm lm ofs1 id i = OK i';
+    }.
+
+Definition globs_inj_into_flatmem (mj:meminj) := 
+  forall b g b' ofs',
+    Genv.find_def ge b = Some g -> 
+    mj b = Some (b', ofs') -> b' = mem_block.
+
+Definition funs_inj_into_flatmem (mj:meminj) := 
+  forall b f b' ofs',
+    Genv.find_funct_ptr ge b = Some (Internal f) -> 
+    mj b = Some (b', ofs') -> b' = mem_block.
+
+Lemma globs_to_funs_inj_into_flatmem : forall (j:meminj),
+    globs_inj_into_flatmem j -> funs_inj_into_flatmem j.
+Proof.
+  unfold globs_inj_into_flatmem, funs_inj_into_flatmem. 
+  unfold Genv.find_funct_ptr. intros.
+  destruct (Genv.find_def ge b) eqn: FDEF; try congruence.
+  destruct g; try congruence. 
+  inv H0. eapply H; eauto.
+Qed.
+
+
+Definition valid_instr_offset_is_internal (mj:meminj) :=
+  forall b f ofs i ofs',
+    Genv.find_funct_ptr ge b = Some (Internal f) ->
+    find_instr (Ptrofs.unsigned ofs) (Asm.fn_code f) = Some i ->
+    mj b = Some (mem_block, ofs') ->
+    Genv.genv_is_instr_internal tge (Ptrofs.add ofs (Ptrofs.repr ofs')) = true.
+
+
+Definition def_frame_inj m := (fun n => if lt_dec n (length (Mem.stack_adt m)) then Some O else None).
+
 Inductive match_states: Asm.state -> FlatAsm.state -> Prop :=
 | match_states_intro: forall (j:meminj) (rs: regset) (m: mem) (rs': regset) (m':mem)
-                        (sj: sectinj) (sm: section_map)
-                        (MINJ: Mem.inject j (fun n => if lt_dec n (length (Mem.stack_adt m)) then Some O else None) m m')
-                        (SMINJ_MATCH: match_sectinj_meminj sj sm j)
+                        (gm: GID_MAP_TYPE) (lm: LABEL_MAP_TYPE) (sm: section_map)
+                        (MINJ: Mem.inject j (def_frame_inj m) m m')
+                        (MATCHSMINJ: match_sminj gm lm sm j)
+                        (GINJFLATMEM: globs_inj_into_flatmem j)
+                        (INSTRINTERNAL: valid_instr_offset_is_internal j)
                         (RSINJ: regset_inject j rs rs'),
     match_states (State rs m) (State rs' m').
 
@@ -51,6 +102,51 @@ Context `{external_calls_ops : !ExternalCallsOps mem }.
 Context `{!EnableBuiltins mem}.
 Existing Instance Asm.mem_accessors_default.
 Existing Instance FlatAsm.mem_accessors_default.
+
+Lemma exec_instr_step : forall j rs1 rs2 m1 m2 rs1' m1' gm lm sm i i' id ofs f,
+    regset_inject j rs1 rs2 ->
+    Mem.inject j (def_frame_inj m1) m1 m2 ->
+    match_sminj gm lm sm j ->
+    RawAsmgen.exec_instr ge f i rs1 m1 = Next rs1' m1' ->
+    transl_instr gm lm ofs id i = OK i' ->
+    exists rs2' m2',
+      FlatAsm.exec_instr tge i' rs2 m2 = Next rs2' m2' /\
+      match_states (State rs1' m1') (State rs2' m2').
+Admitted.
+
+Lemma eval_builtin_arg_inject : forall gm lm sm j m m' rs rs' sp sp' arg varg arg',
+    match_sminj gm lm sm j ->
+    Mem.inject j (def_frame_inj m) m m' ->
+    regset_inject j rs rs' ->
+    Val.inject j sp sp' ->
+    transl_builtin_arg gm arg = OK arg' ->
+    eval_builtin_arg ge rs sp m arg varg ->
+    exists varg', FlatAsmBuiltin.eval_builtin_arg _ _ preg tge rs' sp' m' arg' varg' /\
+             Val.inject j varg varg'.
+Admitted.
+
+Lemma eval_builtin_args_inject : forall gm lm sm j m m' rs rs' sp sp' args vargs args',
+    match_sminj gm lm sm j ->
+    Mem.inject j (def_frame_inj m) m m' ->
+    regset_inject j rs rs' ->
+    Val.inject j sp sp' ->
+    transl_builtin_args gm args = OK args' ->
+    eval_builtin_args ge rs sp m args vargs ->
+    exists vargs', FlatAsmBuiltin.eval_builtin_args _ _ preg tge rs' sp' m' args' vargs' /\
+             Val.inject_list j vargs vargs'.
+Admitted.
+
+
+Lemma external_call_inject : forall j vargs1 vargs2 m1 m2 m1' vres1 t ef,
+    Val.inject_list j vargs1 vargs2 ->
+    Mem.inject j (def_frame_inj m1) m1 m2 ->
+    external_call ef ge vargs1 m1 t vres1 m1' ->
+    exists j' vres2 m2',
+      external_call ef dummy_senv vargs2 m2 t vres2 m2' /\ 
+      Val.inject j' vres1 vres2 /\ Mem.inject j' (def_frame_inj m1') m1' m2' /\
+      inject_incr j j'.
+Admitted.
+      
 
 Theorem step_simulation:
   forall S1 t S2,
@@ -65,11 +161,43 @@ Proof.
   - (* Internal step *)
     unfold regset_inject in RSINJ. generalize (RSINJ Asm.PC). rewrite H. 
     inversion 1; subst.
-
-
+    exploit (agree_sminj_instr gm lm sm j MATCHSMINJ b b2 f ofs delta i); auto.
+    intros (id & i' & ofs1 & FITARG & FSYMB & TRANSL).
+    exploit (globs_to_funs_inj_into_flatmem j); eauto. inversion 1; subst.
+    exploit (exec_instr_step j rs rs'0 m m'0 rs' m' gm lm sm i i' id ofs1 f); auto.
+    intros (rs2' & m2' & FEXEC & MS1).
+    exists (State rs2' m2'). split; auto.
+    apply FlatAsm.exec_step_internal with (Ptrofs.add ofs (Ptrofs.repr delta)) i'; auto.
+    unfold valid_instr_offset_is_internal in INSTRINTERNAL.
+    apply INSTRINTERNAL with b f i; auto.
+        
   - (* Builtin *)
-    admit.
-    
+    unfold regset_inject in RSINJ. generalize (RSINJ Asm.PC). rewrite H.
+    inversion 1; subst.
+    exploit (agree_sminj_instr gm lm sm j MATCHSMINJ b b2 f ofs delta (Asm.Pbuiltin ef args res, sz)); auto.
+    intros (id & i' & ofs1 & FITARG & FSYMB & TRANSL).
+    exploit (globs_to_funs_inj_into_flatmem j); eauto. inversion 1; subst.
+    monadInv TRANSL. monadInv EQ.
+    set (pbsect := {| sect_block_id := code_sect_id; sect_block_start := Ptrofs.repr ofs1; sect_block_size := Ptrofs.repr (si_size sz) |}).
+    fold pbsect in FITARG.
+    exploit (eval_builtin_args_inject gm lm sm j m m'0 rs rs'0 (rs Asm.RSP) (rs'0 Asm.RSP) args vargs x0); auto.
+    intros (vargs' & EBARGS & ARGSINJ).
+    generalize (external_call_inject j vargs vargs' m m'0 m' vres t ef ARGSINJ MINJ H3).
+    intros (j' & vres2 & m2' & EXTCALL & RESINJ & MINJ' & INJINCR).
+    set (rs' := nextinstr_nf (set_res res vres2 (undef_regs (map preg_of (Machregs.destroyed_by_builtin ef)) rs'0)) (sect_block_size pbsect)).
+    exploit (FlatAsm.exec_step_builtin tge (Ptrofs.add ofs (Ptrofs.repr delta))
+                                       ef x0 res rs'0  m'0 vargs' t vres2 rs' m2' pbsect); auto.
+    unfold valid_instr_offset_is_internal in INSTRINTERNAL.
+    eapply INSTRINTERNAL; eauto.
+    intros FSTEP. eexists; split; eauto.
+    eapply match_states_intro with (j:=j'); eauto.
+    (* Supposely the following propreties can proved by separation property of injections *)
+    + admit.
+    + admit.
+    + admit.
+    + subst rs'. unfold regset_inject. intros.
+      admit.
+
   - (* External call *)
     admit.
 
