x86/Sectinj.v
@@ -5,19 +5,11 @@
 
 (** Injection from memory blocks to section lables **)
 
-Require Import Coqlib Integers Maps Values.
+Require Import Coqlib Integers Maps Values AST.
 Require Import Memtype Memory.
 Require Import Sect.
+Require Import Asm.
 Require Import Globalenvs FlatAsmGlobenv FlatAsmgen.
+Require Import Errors.
 
 
-Record match_sm_inj (ge: Asm.genv) (gm: GID_MAP_TYPE) (sm: section_map) (mj: meminj) : Type :=
-  mkMatchSMInj {
-      agree_sm_inj : forall b id sid ofs ofs', 
-        Genv.find_symbol ge id = Some b ->
-        gm id = Some (sid,ofs) -> PTree.get sid sm = Some ofs' -> 
-        mj b = Some (mem_block, Ptrofs.unsigned (Ptrofs.add ofs ofs'));
-      agree_instr : 
-        Genv.find_symbol ge id = Some b ->
-        
-    }.
